rocq/pairing.v
@@ -5,29 +5,28 @@
    demonstrate several advanced tactic uses.  *)
 
 From Stdlib Require Import Lia.
-
 Implicit Types (n x y: nat) (a: nat * nat).
 
-Definition eta a : nat * nat :=
+Definition eta a :=
   match a with
   | (0,y) => (S y, 0)
   | (S x, y) => (x, S y)
   end.
 
-Fixpoint decode n : nat * nat :=
+Fixpoint decode n :=
   match n with
   | 0 => (0,0)
-  | S n' => eta (decode n')
+  | S n => eta (decode n)
   end.
 
-Fixpoint sum n : nat :=
+Fixpoint sigma n :=
   match n with
   | 0 => 0
-  | S n' => S n' + sum n'
+  | S n => sigma n + S n
   end.
 
-Definition encode '(x, y) : nat :=
-  sum (x + y) + y.
+Definition encode '(x, y) :=
+  sigma (x + y) + y.
 
 Fact encode_eta a :
   encode (eta a) = S (encode a).
@@ -65,13 +64,13 @@ Proof.
   revert a.
   enough (forall n a, encode a = n -> decode n = a) by eauto.
   induction n as [|n IH]; cbn; intros a.
-  - destruct a as [[|x] [|y]]; cbn; easy.
+  - destruct a as [[|x] [|y]]; cbn; (lia || easy).
   - destruct (eta_pi a) as [-> | ->]; cbn. easy.
     rewrite encode_eta. intros [= H1%IH]. congruence.
 Qed.
 
 Fact Gauss n :
-  2 * sum n = n * S n.
+  2 * sigma n = n * S n.
 Proof.
   induction n as [|n IH]; cbn; lia.
 Qed.
